src/3d/prelude/EverParse3d.InputStream.Base.fst
@@ -106,6 +106,25 @@ class input_stream_inst (t: Type) : Type = {
       get_remaining x h' `Seq.equal` Seq.slice s (U64.v n) (Seq.length s)
     ));
 
+  skip_if_success:
+    (x: t) ->
+    (pos: LPE.pos_t) ->
+    (res: U64.t) ->
+    HST.Stack unit
+    (requires (fun h ->
+      live x h /\
+      (LPE.is_success res ==> (
+        U64.v pos == Seq.length (get_read x h)) /\
+        U64.v res >= U64.v pos /\
+        U64.v pos + Seq.length (get_remaining x h) >= U64.v res
+    )))
+    (ensures (fun h _ h' ->
+      let s = get_remaining x h in
+      B.modifies (footprint x) h h' /\
+      live x h' /\
+      get_remaining x h' == (if LPE.is_success res then Seq.slice s (U64.v res - U64.v pos) (Seq.length s) else get_remaining x h)
+    ));
+
   empty:
     (x: t) ->
     (pos: LPE.pos_t) ->
